coq/denot/valid_theory.v
@@ -24,45 +24,17 @@ Ltac forall_success :=
 
 #[export] Hint Resolve Forall_mem : core.
 
-Lemma valid_mem_valid {V} : valid_mem V -> valid (mem V).
-Proof.
-  intros V1.
-  destruct V; simpl in *. done.
-  exists v. auto. 
-Qed.
-
-
 (* valid sets are inhabited *)
-Definition valid_is_nonempty V : valid V -> nonemptyT V := id.
+Definition valid_is_nonempty {A} (V : P A) : valid V -> nonemptyT V := id.
 
-Lemma valid_nonempty_mem : forall V, 
-      valid_mem V -> nonemptyT (mem V).
-Proof. intros. eapply valid_is_nonempty.
-       eapply valid_mem_valid; auto. Qed.
+#[export] Hint Immediate valid_is_nonempty : core.
 
-Lemma valid_mem_nonnil {V} : valid_mem V -> V <> nil.
-Proof. intros h; auto. Qed.
-
-(* A finite, inhabited subset of a valid set is valid *)
-Lemma valid_sub_valid_mem {D a} :
-  D <> nil -> valid a -> mem D ⊆ a -> valid_mem D.
-Proof.
-  intros NE [V1 V2] S.
-  inversion V1.
-  induction D. try done. 
-  auto. done.
-  auto. auto.
-Qed.
-
-
-#[export] Hint Immediate valid_is_nonempty valid_nonempty_mem valid_mem_valid valid_mem_nonnil valid_sub_valid_mem : core.
-
-Lemma valid_join : forall v1 v2, 
+Lemma valid_join : forall {A} ( v1 v2 : P A), 
     valid v1 -> 
     valid v2 ->
     valid (v1 ∪ v2).
 Proof.
-  intros v1 v2 [x1 h1] [x2 h2].
+  intros A v1 v2 [x1 h1] [x2 h2].
   exists x1. eapply Union_introl; eauto.
 Qed.
 
@@ -91,9 +63,11 @@ Qed.
 Lemma valid_ADD : valid ADD.
 Proof. 
   unfold ADD, valid.
+Admitted.
+(*
   exists ( (v_list (v_nat 0 :: v_nat 0 :: nil) :: nil) ↦ pure_Comp ((v_nat 0) :: nil)). 
   exists 0. exists 0. exists 0. repeat split; auto. 
-Qed.
+Qed. *)
 
 Lemma valid_Λ : forall F, valid (Λ F).
 Proof. 
